sel4_artifacts/UxASSeL4/components/Waypoint_Manager/include/mcutils.h
@@ -1,0 +1,76 @@
+#ifndef __MCUTILS_H__
+#define __MCUTILS_H__
+#include <stdint.h>
+#include <stdio.h>
+#include <stdbool.h>
+
+#define WP_HDR_LEN 15
+
+struct  __attribute__((packed)) wp_struct {
+  char header[WP_HDR_LEN];
+  uint64_t /*double*/ latitude;
+  uint64_t /*double*/ longitude;
+  uint32_t /*float*/ altitude;
+  int32_t altitude_type;
+  uint64_t id;
+  uint64_t nxid;
+  uint32_t /*float*/ speed;
+  int32_t speed_type;
+  float climbrate;
+  int32_t turntype;
+  uint16_t vehicleactionlistsize;
+  uint64_t contingencywaypointa;
+  uint64_t contingencywaypointb;
+  uint16_t associatedtasksize;
+};
+
+typedef struct wp_struct wp_t;
+
+#define MC_HDR_LEN 23
+ 
+struct __attribute__((packed)) mc_trnc_struct {
+  char header[MC_HDR_LEN];
+  uint64_t commandid;
+  uint64_t vehicleid;
+  uint16_t vehicleactionlistsize;
+  int32_t commandstatus;
+  uint16_t waypointssize;
+};
+
+typedef struct mc_trnc_struct mc_trnc_t;
+
+#define MAX_WAYPOINTS 255
+
+struct __attribute__((packed)) mc_full_struct {
+  char header[MC_HDR_LEN];
+  uint64_t commandid;
+  uint64_t vehicleid;
+  uint16_t vehicleactionlistsize;
+  int32_t commandstatus;
+  uint16_t waypointssize;
+  wp_t waypoints[MAX_WAYPOINTS];
+  uint64_t startingwaypoint;
+  uint32_t checksum;
+};
+
+typedef struct mc_full_struct mc_full_t;
+
+union mc_union {
+  mc_trnc_t trnc;
+  mc_full_t full;
+};
+
+typedef union mc_union mc_t;
+
+bool DeserializeMCFromBuffer(const uint8_t * buf, mc_t * mc_ptr);
+
+bool DeserializeMCFromFile(FILE * f, mc_t * mc_ptr);
+
+void PrintMC(FILE * f, mc_t * mc_ptr);
+
+bool MCPrefix(const mc_t * orig_mc_ptr,
+              const uint64_t id,
+              const uint16_t len,
+              mc_t * mc_new_ptr);
+
+#endif /* __MCUTILS_H__ */
