sel4_artifacts/UxASSeL4/components/Waypoint_Manager/src/waypoint_manager.c
@@ -1,22 +1,91 @@
 #include <stdio.h>
+#include <strings.h>
 #include <tb_Waypoint_Manager.h>
+#include <camkes.h>
+#include <mcutils.h>
+
+#define MAX_AP_WAYPOINTS 8
+#define DEBUG(fmt,args...)   printf("%s,%s,%i:"fmt,__FUNCTION__,"waypoint_manager.c",__LINE__,##args)
+
+#define UART_PACKET_SZ 255
+
+#define MC_SZ(waypoints) (sizeof(mc_t)-(MAX_WAYPOINTS*sizeof(wp_t))+(waypoints*sizeof(wp_t)))
+
+static bool valid_mc = false;
+static mc_t mc = {};
+static mc_t swin = {};
+
+static bool valid_nw = false;
+static mc_t nw = {};
+
+
 
 void component_entry(const int64_t * periodic_dispatcher) {
-
+  //DEBUG("Periodic execution.\n");
 }
 
 void component_init(const int64_t *arg) {
-
+  DEBUG("Starting Waypoint_Manager.\n");
 }
 
-void mission_write(const uint32_t * tb_mission_write) {
-    printf("WM saw mission right from the VM\n");
-    uint32_t numBytes = 42;
-    mission_read(&numBytes);
+static void send_swin() {
+  SMACCM_DATA__UART_Packet_i packet;
+  size_t pkts = MC_SZ(swin.full.waypointssize)/UART_PACKET_SZ;
+  for(size_t i = 0; i < pkts; i++) {
+    DEBUG("Packing and sending packet %u/%u.\n",i,pkts);
+    packet.buf_len = UART_PACKET_SZ;
+    memcpy(packet.buf,((char*)(&swin))+(UART_PACKET_SZ*i),UART_PACKET_SZ);
+    assert(out_uart_packet(&packet) == true);
+  }
+  size_t remaining = MC_SZ(swin.full.waypointssize) % UART_PACKET_SZ;
+  if( remaining > 0) {
+    DEBUG("Packing and sending remianing %u bytes.\n",remaining);    
+    packet.buf_len = remaining;
+    memcpy(packet.buf,((char*)(&swin))+(UART_PACKET_SZ*pkts),remaining);
+    assert(out_uart_packet(&packet) == true);
+  }
 }
 
-void waypoint_write(const uint32_t * tb_waypoint_write) {
-	printf("%i:%s:%s",__LINE__,__FILE__,__FUNCTION__);
+void mission_write(const bool * _UNUSED) {
+  DEBUG(" Entry.\n");
+  if(DeserializeMCFromBuffer((uint8_t *)mission, &mc) != true) {
+    DEBUG(" Failed to deserialize buffer.\n");
+  } else {
+    mission_read(_UNUSED);
+    valid_mc = true;
+    DEBUG("Begin mission command output.\n");
+    PrintMC(stdout,&mc);
+    DEBUG("End mission command output.\n");
+    assert(MCWaypointSubSequence(&mc,
+                                 mc.full.startingwaypoint,
+                                 MAX_AP_WAYPOINTS,
+                                 &swin) == true);
+    DEBUG("Intial waypoint window created.\n");
+    DEBUG("Sending initial window.\n");
+    send_swin();
+    DEBUG("Initial window tranmission complete.\n");
+    
+    //TODO: Send the first sliding window to the AP.
+  }
+  DEBUG(" Exit.\n");
+  
+  return;
+}
+
+void waypoint_write(const bool * _UNUSED) {
+  DEBUG(" Entry.");
+  if(DeserializeMCFromBuffer((uint8_t *)mission, &nw) != true) {
+    DEBUG(" Failed to deserialize buffer.");
+  } else {
+    mission_read(_UNUSED);
+    valid_nw = true;
+    DEBUG("\nBegin next waypoint output.\n");
+    PrintMC(stdout,&nw);
+    DEBUG("\nEnd next waypoint output.\n");
+    //TODO: Get the waypoint the asset is currently heading towards.
+  }
+  DEBUG(" Exit.");
+  return;
 }
 
 
