src/Services/Waypoint2Sel4Service.cpp
@@ -45,112 +45,112 @@
 
 namespace uxas
 {
-namespace service
-{
-Waypoint2Sel4Service::ServiceBase::CreationRegistrar<Waypoint2Sel4Service>
-Waypoint2Sel4Service::s_registrar(Waypoint2Sel4Service::s_registryServiceTypeNames());
+  namespace service
+  {
+    Waypoint2Sel4Service::ServiceBase::CreationRegistrar<Waypoint2Sel4Service>
+    Waypoint2Sel4Service::s_registrar(Waypoint2Sel4Service::s_registryServiceTypeNames());
 
-Waypoint2Sel4Service::Waypoint2Sel4Service()
-: ServiceBase(Waypoint2Sel4Service::s_typeName(), Waypoint2Sel4Service::s_directoryName()) { };
+    Waypoint2Sel4Service::Waypoint2Sel4Service()
+      : ServiceBase(Waypoint2Sel4Service::s_typeName(), Waypoint2Sel4Service::s_directoryName()) { };
 
-Waypoint2Sel4Service::~Waypoint2Sel4Service() { };
+    Waypoint2Sel4Service::~Waypoint2Sel4Service() { };
 
-bool
-Waypoint2Sel4Service::configure(const pugi::xml_node& ndComponent)
-{
-    m_vehicleID = m_entityId; // can be overridden below
-
-    if (!ndComponent.attribute(STRING_XML_VEHICLE_ID).empty())
+    bool
+    Waypoint2Sel4Service::configure(const pugi::xml_node& ndComponent)
     {
-        m_vehicleID = ndComponent.attribute(STRING_XML_VEHICLE_ID).as_uint();
+      m_vehicleID = m_entityId; // can be overridden below
+
+      if (!ndComponent.attribute(STRING_XML_VEHICLE_ID).empty())
+        {
+          m_vehicleID = ndComponent.attribute(STRING_XML_VEHICLE_ID).as_uint();
+        }
+
+      addSubscriptionAddress(afrl::cmasi::AutomationResponse::Subscription);
+      addSubscriptionAddress(afrl::cmasi::MissionCommand::Subscription); 
+      return true;
     }
 
-    addSubscriptionAddress(afrl::cmasi::AutomationResponse::Subscription);
-    addSubscriptionAddress(afrl::cmasi::MissionCommand::Subscription); 
-    return true;
-}
-
-bool Waypoint2Sel4Service::initialize()
-{
-    return true;
-}
-
-
-bool Waypoint2Sel4Service::start()
-{
-    COUT_INFO("Started\n");
-    return true;
-}
-
-
-bool Waypoint2Sel4Service::terminate()
-{
-    return true;
-}
-
-void Waypoint2Sel4Service::write2Sel4(afrl::cmasi::MissionCommand * mission){
-    uint32_t i;
-    uint8_t * pArray;
-
-    COUT_INFO("in write2Sel4\n");
-
-    if (mission->getVehicleID() == m_vehicleID)
+    bool Waypoint2Sel4Service::initialize()
     {
-        mission->getVehicleActionList().clear();
-        auto waypointList = mission->getWaypointList();
-        for(auto waypoint : waypointList){
+      return true;
+    }
+
+
+    bool Waypoint2Sel4Service::start()
+    {
+      COUT_INFO("Started\n");
+      return true;
+    }
+
+
+    bool Waypoint2Sel4Service::terminate()
+    {
+      return true;
+    }
+
+    void Waypoint2Sel4Service::write2Sel4(afrl::cmasi::MissionCommand * mission){
+      uint32_t i;
+      uint8_t * pArray;
+
+      COUT_INFO("in write2Sel4\n");
+
+      if (mission->getVehicleID() == m_vehicleID)
+        {
+          mission->getVehicleActionList().clear();
+          auto waypointList = mission->getWaypointList();
+          for(auto waypoint : waypointList){
             waypoint->getVehicleActionList().clear();
             waypoint->getAssociatedTasks().clear();
-        }
-        avtas::lmcp::ByteBuffer* buf = avtas::lmcp::Factory::packMessage(mission, true);
-        #if 1 == 1
-        int fd = open("/dev/mem", O_RDWR | O_SYNC);
-        uint8_t * mem = (uint8_t *)mmap(0, 1, PROT_READ | PROT_WRITE, MAP_SHARED, fd, 0xE0000000);
+          }
+          avtas::lmcp::ByteBuffer* buf = avtas::lmcp::Factory::packMessage(mission, true);
+#if 1 == 1
+          int fd = open("/dev/mem", O_RDWR | O_SYNC);
+          uint8_t * mem = (uint8_t *)mmap(0, 1, PROT_READ | PROT_WRITE, MAP_SHARED, fd, 0xE0000000);
 
-	COUT_INFO(mission->toString());
-        COUT_INFO("Capacity: ");
-        COUT_INFO(buf->capacity());
-	pArray = buf->array();
-	for(i = 0; i < buf->capacity(); i++){
+          COUT_INFO(mission->toString());
+          COUT_INFO("Capacity: ");
+          COUT_INFO(buf->capacity());
+          pArray = buf->array();
+          for(i = 0; i < buf->capacity(); i++){
             *mem = *(pArray++);
-	}
-//        buf->rewind();
-//        while(buf->hasRemaining()){
-//            *mem = buf->get();
-//        }
+          }
+          //        buf->rewind();
+          //        while(buf->hasRemaining()){
+          //            *mem = buf->get();
+          //        }
 
-        close(fd);
-        #else
-        FILE * f = fopen("/tmp/missioncommands", "wb");
-        fwrite(buf->array(),1,buf->capacity(),f);
-        fclose(f);
-        #endif
-        delete buf;
-    }
-}
-
-bool
-Waypoint2Sel4Service::processReceivedLmcpMessage(std::unique_ptr<uxas::communications::data::LmcpMessage> receivedLmcpMessage)
-{
-
-    COUT_INFO("Got message!\n");
-    if (afrl::cmasi::isAutomationResponse(receivedLmcpMessage->m_object))
-    {
-        auto automationResponse = std::static_pointer_cast<afrl::cmasi::AutomationResponse> (receivedLmcpMessage->m_object);
-        for (auto mission : automationResponse->getMissionCommandList())
-        {
-	    COUT_INFO("Writing message!\n");
-            write2Sel4(mission);
+          close(fd);
+#else
+          FILE * f = fopen("/tmp/missioncommands", "wb");
+          fwrite(buf->array(),1,buf->capacity(),f);
+          fclose(f);
+#endif
+          delete buf;
         }
     }
-    else if (afrl::cmasi::isMissionCommand(receivedLmcpMessage->m_object))
-    {
-        auto mission = std::static_pointer_cast<afrl::cmasi::MissionCommand> (receivedLmcpMessage->m_object);
-	COUT_INFO("Writing message!\n");
-        write2Sel4(mission.get());
-    }
-    return (false); // always false implies never terminating service from here
-}
 
-}; //namespace service
+    bool
+    Waypoint2Sel4Service::processReceivedLmcpMessage(std::unique_ptr<uxas::communications::data::LmcpMessage> receivedLmcpMessage)
+    {
+
+      COUT_INFO("Got message!\n");
+      if (afrl::cmasi::isAutomationResponse(receivedLmcpMessage->m_object))
+        {
+          auto automationResponse = std::static_pointer_cast<afrl::cmasi::AutomationResponse> (receivedLmcpMessage->m_object);
+          for (auto mission : automationResponse->getMissionCommandList())
+            {
+              COUT_INFO("Writing message!\n");
+              write2Sel4(mission);
+            }
+        }
+      else if (afrl::cmasi::isMissionCommand(receivedLmcpMessage->m_object))
+        {
+          auto mission = std::static_pointer_cast<afrl::cmasi::MissionCommand> (receivedLmcpMessage->m_object);
+          COUT_INFO("Writing message!\n");
+          write2Sel4(mission.get());
+        }
+      return (false); // always false implies never terminating service from here
+    }
+
+  }; //namespace service
 }; //namespace uxas
